P1.fsti
@@ -8,6 +8,7 @@ open Steel.Reference
 
 module Spec = Trees
 module U = FStar.UInt64
+module I = FStar.Int64
 
 #set-options "--ide_id_info_off"
 
@@ -15,6 +16,11 @@ inline_for_extraction noextract
 let one = U.uint_to_t 1
 inline_for_extraction noextract
 let zero = U.uint_to_t 0
+
+inline_for_extraction noextract
+let sone = I.int_to_t 1
+inline_for_extraction noextract
+let szero = I.int_to_t 0
 
 val create_leaf (#a: Type0) (_: unit) : Steel (t a)
   emp (fun ptr -> linked_tree ptr)
@@ -94,6 +100,30 @@ val member (#a: eqtype) (ptr: t a) (v: a)
     (ensures fun h0 b h1 ->
         v_linked_tree ptr h0 == v_linked_tree ptr h1 /\
         (Spec.mem (v_linked_tree ptr h0) v <==> b))
+
+type cmp (a: Type) = compare: (a -> a -> I.t){
+  squash (forall x. I.eq (compare x x) I.zero) /\
+  squash (forall x y. I.gt (compare x y) I.zero
+                 <==> I.lt (compare y x) I.zero) /\
+  squash (forall x  y z. I.gte (compare x y) I.zero /\
+                         I.gte (compare y z) I.zero /\
+                         I.gte (compare x z) I.zero)
+}
+
+let convert (#a: Type) (cmp: cmp a) : GTot (Spec.cmp a)
+  = fun x y -> I.v (cmp x y)
+
+val insert_bst (#a: Type0) (cmp:cmp a) (ptr:t a) (v: a)
+  : Steel (t a)
+  (linked_tree ptr)
+  (fun ptr' -> linked_tree ptr')
+  (requires fun h0 ->
+    Spec.size_of_tree (v_linked_tree ptr h0) < c - 1 /\
+    Spec.is_bst (convert cmp) (v_linked_tree ptr h0))
+  (ensures fun h0 ptr' h1 ->
+    Spec.is_bst (convert cmp) (v_linked_tree ptr h0) /\
+    Spec.insert_bst (convert cmp) (v_linked_tree ptr h0) v
+    == v_linked_tree ptr' h1)
 
 (*** Rotation functions used internally to balance AVL trees ***)
 
